# Simplifying Difference of Expanded Squares

## General Pattern

When subtracting one expanded square from another: **(a+b)² - (c+d)²**

The key steps:
1. Expand both squares completely using (a+b)² = a² + 2ab + b²
2. Distribute the negative sign carefully through the second expansion
3. Collect like terms by grouping x², x, and constant terms

## Worked Example: (2x + 3)² - (x - 1)²

This is a perfect example for solving equations like (2x + 3)² - (x - 1)² = 45.

### Step 1: Expand the first square

(2x + 3)² = (2x)² + 2(2x)(3) + 3²
         = 4x² + 12x + 9

### Step 2: Expand the second square

(x - 1)² = x² - 2(x)(1) + 1²
         = x² - 2x + 1

### Step 3: Subtract with careful attention to signs

4x² + 12x + 9 - (x² - 2x + 1)

**Critical**: The negative sign distributes to ALL terms inside the parentheses!

= 4x² + 12x + 9 - x² + 2x - 1

Notice how -2x becomes +2x when we distribute the negative.

### Step 4: Collect like terms

Group by degree:

**x² terms**: 4x² - x² = 3x²

**x terms**: 12x + 2x = 14x

**Constants**: 9 - 1 = 8

**Final Result**: 3x² + 14x + 8

## Common Mistakes

### Mistake 1: Forgetting to distribute the negative

**WRONG**: (2x+3)² - (x-1)² = 4x² + 12x + 9 - x² - 2x + 1 ❌

This keeps -2x instead of changing it to +2x!

**RIGHT**: 4x² + 12x + 9 - x² **+ 2x** - 1 ✓

### Mistake 2: Arithmetic errors when collecting terms

**WRONG**: 12x + 2x = 10x ❌

**RIGHT**: 12x + 2x = 14x ✓

Always double-check your arithmetic!

## Another Example: (3x + 1)² - (2x - 2)²

### Step 1: Expand both squares
- (3x + 1)² = 9x² + 6x + 1
- (2x - 2)² = 4x² - 8x + 4

### Step 2: Subtract
9x² + 6x + 1 - (4x² - 8x + 4)
= 9x² + 6x + 1 - 4x² + 8x - 4

### Step 3: Collect terms
- x² terms: 9x² - 4x² = 5x²
- x terms: 6x + 8x = 14x
- Constants: 1 - 4 = -3

**Result**: 5x² + 14x - 3

## Verification Strategy

Always verify by checking one value. If x = 1:

**Original**: (3(1)+1)² - (2(1)-2)² = 4² - 0² = 16
**Simplified**: 5(1)² + 14(1) - 3 = 5 + 14 - 3 = 16 ✓

## Application to Equations

If we have (2x + 3)² - (x - 1)² = 45, we now know the left side simplifies to:

3x² + 14x + 8 = 45

Rearranging: 3x² + 14x - 37 = 0

This is now a standard quadratic equation ready to solve!
