# Expanding Squared Binomials

## Pattern: (a + b)²

The expansion formula for a squared binomial is:

**(a + b)² = a² + 2ab + b²**

This is NOT just a² + b²! The middle term 2ab is crucial.

### With Coefficients

When expanding (2x + 3)²:

**Step 1**: Identify a and b
- a = 2x
- b = 3

**Step 2**: Apply the formula
- (2x)² = 4x²
- 2(2x)(3) = 12x
- 3² = 9

**Step 3**: Combine
(2x + 3)² = 4x² + 12x + 9

### Common Mistake

**WRONG**: (2x + 3)² = 4x² + 9 ❌

**RIGHT**: (2x + 3)² = 4x² + 12x + 9 ✓

The middle term 2(2x)(3) = 12x cannot be skipped!

## Pattern: (a - b)²

The expansion formula with subtraction:

**(a - b)² = a² - 2ab + b²**

Notice the middle term is negative but the last term is positive.

### Example: (x - 1)²

**Step 1**: Identify a and b
- a = x
- b = 1

**Step 2**: Apply the formula
- x² = x²
- -2(x)(1) = -2x
- 1² = 1

**Step 3**: Combine
(x - 1)² = x² - 2x + 1

### Important Rules

1. The first term is always positive (squaring is always positive)
2. The middle term has the sign from the binomial
3. The last term is always positive (squaring is always positive)

## Worked Example 1

**Problem**: Expand (3x + 2)²

**Solution**:
1. Identify: a = 3x, b = 2
2. Apply formula: (3x)² + 2(3x)(2) + 2²
3. Calculate each term:
   - (3x)² = 9x²
   - 2(3x)(2) = 12x
   - 2² = 4
4. **Answer**: 9x² + 12x + 4

## Worked Example 2

**Problem**: Expand (2y - 5)²

**Solution**:
1. Identify: a = 2y, b = 5
2. Apply formula: (2y)² - 2(2y)(5) + 5²
3. Calculate each term:
   - (2y)² = 4y²
   - -2(2y)(5) = -20y
   - 5² = 25
4. **Answer**: 4y² - 20y + 25

## Practice Pattern Recognition

- (x + 4)² = x² + 8x + 16
- (5x + 1)² = 25x² + 10x + 1
- (x - 3)² = x² - 6x + 9
- (4x - 2)² = 16x² - 16x + 4

The middle coefficient is always 2 times the product of the original terms!
